

# MATH 273 - Lecture 11 (09/30/2014)

11.1

## Estimating changes in a specific direction

In 1D, change in  $f(x)$  at  $x=p_0$  is estimated by

$$df = \underbrace{f'(p_0)}_{\substack{\downarrow \\ \text{differential of } f \text{ at } x=p_0}} \cdot \underbrace{dx}_{\text{derivative } \times \text{ increment}}$$

Extending to higher dimensions,

$$df = ((\nabla f)_{p_0} \cdot \hat{u}) ds, \quad \text{where } ds \text{ is the change in the direction of } \hat{u}.$$

directional derivative  $\times$  increment in the direction of  $\hat{u}$

Prob 21 By about how much will  $g(x,y,z) = x + x \cos z - y \sin z + y$  change when  $P(x,y,z)$  moves from  $P_0(2,-1,0)$  toward the point  $P_1(0,1,2)$  a distance of  $ds=0.2$  units?

$$\begin{aligned} \nabla g &= \frac{\partial g}{\partial x} \hat{i} + \frac{\partial g}{\partial y} \hat{j} + \frac{\partial g}{\partial z} \hat{k} \\ &= (1 + \cos z - 0 + 0) \hat{i} + (0 + 0 - \sin z + 1) \hat{j} + (0 - x \sin z - y \cos z + 0) \hat{k} \\ &= (1 + \cos z) \hat{i} + (1 - \sin z) \hat{j} - (x \sin z + y \cos z) \hat{k} \\ (\nabla g)_{P_0} &= (1 + \underbrace{\cos 0}_1) \hat{i} + (1 - \underbrace{\sin 0}_0) \hat{j} - (2 \underbrace{\sin 0}_0 + (-1) \underbrace{\cos 0}_1) \hat{k} \\ &= 2 \hat{i} + \hat{j} + \hat{k}. \end{aligned}$$

Direction  $\bar{u} = \overrightarrow{P_0 P_1} = (0-2)\hat{i} + (1-1)\hat{j} + (2-0)\hat{k}$   
 $= -2\hat{i} + 2\hat{j} + 2\hat{k}$

$$P_0(2, -1, 0)$$

$$P_1(0, 1, 2)$$

$$\|\bar{u}\| = \sqrt{(-2)^2 + (2)^2 + (2)^2} = 2\sqrt{3}.$$

$$\text{So, } \hat{u} = \frac{\bar{u}}{\|\bar{u}\|} = \frac{1}{2\sqrt{3}}(-2\hat{i} + 2\hat{j} + 2\hat{k}) = \frac{1}{\sqrt{3}}(-\hat{i} + \hat{j} + \hat{k}).$$

$$\begin{aligned} (D_{\hat{u}}g)_{P_0} &= (\nabla g)_{P_0} \cdot \hat{u} = (2\hat{i} + \hat{j} + \hat{k}) \cdot \frac{1}{\sqrt{3}}(-\hat{i} + \hat{j} + \hat{k}) \\ &= \frac{1}{\sqrt{3}}(2 \times -1 + 1 \times 1 + 1 \times 1) = 0. \end{aligned}$$

$$\text{So } dg = (D_{\hat{u}}g)_{P_0} \cdot ds = 0 \cdot (0.2) = 0.$$

# Review for Exam 1

Exam 1 covers 13.1, 13.3, 13.4, and 13.5.

domain, range,  
level curves, open/closed,  
bounded/unbounded

partial  
derivatives

chain rule  
branch diagrams

gradient &  
directional  
derivative

## Practice Exam

(8) True/False

(a) False. Take  $y \geq x^2$  is closed, as it includes its boundary  $y = x^2$ . But it is unbounded



(b) False. We draw two branch diagrams, one for each independent variable.

(c) True. Follows from properties of  $\nabla f$ .

(d) False.  $(D_{\hat{u}}f) = \nabla f \cdot \hat{u} = |\nabla f| \underbrace{|\hat{u}|}_{=1} \cos \theta$

If  $|\nabla f| = 0$ , then  $(D_{\hat{u}}f) = 0$  in all directions  $\hat{u}$ .

$$2(a). \quad f(x, y) = \frac{x+y}{xy-1}$$

$$\frac{\partial f}{\partial x} = \frac{(xy-1)(1+0) - (x+y)(y-0)}{(xy-1)^2} = \frac{\cancel{xy}-1 - \cancel{xy}-y^2}{(xy-1)^2} = \frac{-(y^2+1)}{(xy-1)^2}$$

$f(x, y)$  is symmetric w.r.t  $x$  and  $y$ , so

$$\frac{\partial f}{\partial y} = \frac{-(x^2+1)}{(yx-1)^2} = \frac{-(x^2+1)}{(xy-1)^2}. \quad f(y, x) = \frac{y+x}{yx-1} = \frac{x+y}{xy-1} = f(x, y)$$

Alternatively, we could evaluate  $\frac{\partial f}{\partial y}$  directly:

$$\begin{aligned} \frac{\partial f}{\partial y} &= \frac{(xy-1)(0+1) - (x+y)(x-0)}{(xy-1)^2} = \frac{\cancel{(xy-1)} - x^2 - \cancel{xy}}{(xy-1)^2} \\ &= \frac{-(x^2+1)}{(xy-1)^2}. \end{aligned}$$